@prefix : <https://w3id.org/mint/dataCatalog#> .
@prefix geo-lower-abstraction: <http://www.geoscienceontology.org/geo-lower/abstraction#> .
@prefix geo-lower-variable: <http://www.geoscienceontology.org/geo-lower/variable#> .
@prefix geo-upper: <http://www.geoscienceontology.org/geo-upper#> .
@prefix cf: <http://purl.oclc.org/NET/ssnx/cf/cf-feature#> .
@prefix owl: <http://www.w3.org/2002/07/owl#> .
@prefix skos: <http://www.w3.org/2004/02/skos/core#>.
@prefix rdf: <http://www.w3.org/1999/02/22-rdf-syntax-ns#> .
@prefix xml: <http://www.w3.org/XML/1998/namespace> .
@prefix xsd: <http://www.w3.org/2001/XMLSchema#> .
@prefix rdfs: <http://www.w3.org/2000/01/rdf-schema#> .
@prefix dcat: <http://www.w3.org/ns/dcat#> .
@prefix om: <http://www.ontology-of-units-of-measure.org/resource/om-2/> .
@prefix cco: <http://www.ontologyrepository.com/CommonCoreOntologies/> .
@prefix qudt: <http://qudt.org/1.1/vocab/> .
@base <https://w3id.org/mint/dataCatalog> .

<https://w3id.org/mint/dataCatalog> rdf:type owl:Ontology ;
                                      owl:versionIRI <https://w3id.org/mint/dataCatalog/0.1.0> ;
                                      <http://purl.org/dc/elements/1.1/contributor> "Daniel Garijo"@en ,
										  											"Yao-Yi Chiang"@en ,
																					"Binh Vu"@en ,
										  											"Craig Knoblock"@en,
																					"Arunkumar Rajendran"@en,
																					"Dan Feldman"@en;
                                      <http://purl.org/dc/elements/1.1/creator> "Jay Pujara"@en ;
                                      <http://purl.org/dc/elements/1.1/license> "http://creativecommons.org/licenses/by/2.0/"@en ;
                                      <http://purl.org/dc/elements/1.1/title> "The MINT Data Catalog Ontology"@en ;
                                      <http://purl.org/vocab/vann/preferredNamespacePrefix> "datacatalog"@en ;
                                      rdfs:comment "An ontology for describing datasets, the variables they contain, and other representational details."@en ;
		                              owl:imports <http://www.geoscienceontology.org/geo-upper> ,
		                                          <http://www.w3.org/ns/dcat> ;
                                      owl:versionInfo "0.1.0"^^xsd:string .

#################################################################
#    Object Properties
#################################################################

:hasCKANid rdf:type owl:ObjectProperty ;
			rdfs:label "has CKAN id"@en ;
			rdfs:comment "A mapping from a dataset to a CKAN identifier"@en ;
			rdfs:domain :Dataset ;
			rdfs:range :CKANIdentifier .


:hasDataOffset rdf:type owl:ObjectProperty ;
			rdfs:label "has data offset"@en ;
			rdfs:comment "Specifies the location of a variable in a file"@en ;
			rdfs:domain :Presentation ;				 
			rdfs:range :DataOffset .

:hasDataset rdf:type owl:ObjectProperty ;
			rdfs:label "has dataset"@en ;
			rdfs:comment "Associates a presentation with a dataset where the presentation occurs"@en ;
			rdfs:domain :Presentation ;
			rdfs:range :Dataset .

:hasStandardName rdf:type owl:ObjectProperty ;
			rdfs:label "has standard name"@en ;
			rdfs:comment "The standard name of a variable contained in the data catalog"@en ;
			rdfs:domain :Variable ;
			rdfs:range :StandardName .

:hasStoragePath rdf:type owl:ObjectProperty ;
			rdfs:label "has storage path"@en ;
			rdfs:comment "Associates a dataset with its storage path"@en ;
			rdfs:domain :Dataset ;
			rdfs:range :StoragePath .

:hasVariable rdf:type owl:ObjectProperty ;
			rdfs:label "has variable"@en ;
			rdfs:comment "Associates a presentation with the variable the presentation represents"@en ;
			rdfs:domain :Presentation ;
			rdfs:range :Variable .

:inDataset rdf:type owl:ObjectProperty ;
			rdfs:label "in dataset"@en ;
			rdfs:comment "Associates a variable with a dataset that includes the variable"@en ;
            rdfs:domain :Variable ;
            rdfs:range :Dataset .


:usesAggregationMethod rdf:type owl:ObjectProperty ;
			rdfs:label "uses aggregation method"@en ;
			rdfs:comment "Records the aggregation method used to combine data points or resample data"@en ;
			rdfs:domain :Presentation ;
			rdfs:range :AggregationMethod .


:usesMissingValueIndicator rdf:type owl:ObjectProperty ;
			rdfs:label "uses missing value indicator"@en ;
			rdfs:comment "Records the missing value indicator or approach in a presentation"@en ;
			rdfs:domain :Presentation ;
			rdfs:range :MissingValueIndicator .

:usesTimeConvention rdf:type owl:ObjectProperty ;
			rdfs:label "uses time convention"@en ;
			rdfs:comment "Records the time convention used by a presentation"@en ;
			rdfs:domain :Presentation ;
			rdfs:range :TimeConvention .

:usesUnit rdf:type owl:ObjectProperty ;
			rdfs:label "uses Unit"@en ;
			rdfs:comment "Records the unit of measurement used by a presentation"@en ;
			rdfs:domain :Presentation ;
			rdfs:range  [ rdf:type owl:Class ;
							owl:unionOf (	cco:MeasurementUnit 
											qudt:Unit
										)
						] .


#################################################################
#    Data properties
#################################################################
:hasDescription rdf:type owl:DatatypeProperty ;
			rdfs:label "has description"@en ;
			rdfs:comment "A human-readable description of a variable, which may include additional contextual information used to map to a standard name"@en ;
			rdfs:domain :Variable ;
			rdfs:range xsd:string .

:hasShortName rdf:type owl:DatatypeProperty ;
			rdfs:label "has short name"@en ;
			rdfs:comment "A short name (e.g., temperature) capturing the high-level concept of the variable"@en ;
			rdfs:domain :Variable ;
			rdfs:range xsd:string .

:hasSpatialDescription rdf:type owl:DatatypeProperty ;
			rdfs:label "has spatial description"@en ;
			rdfs:comment "A human-readable description of the spatial region (e.g., South Sudan or Hudson River Valley) the dataset encompasses"@en ;
			rdfs:domain :Dataset ;
			rdfs:range xsd:string .

:usesScale rdf:type owl:DatatypeProperty ;
			rdfs:label "uses scale"@en ;
			rdfs:comment "A numerical value for the scale used in measurements"@en ;
            rdfs:domain :Presentation ;
            rdfs:range xsd:float .

:usesSpatialResolution rdf:type owl:DatatypeProperty ;
			rdfs:label "uses spatial resolution"@en ;
			rdfs:comment "A numerical value for the spatial resolution data is recorded at in a dataset"@en ;
			rdfs:domain :Dataset ;
			rdfs:range xsd:float .


#################################################################
#    Classes
#################################################################
:AggregationMethod rdf:type owl:Class ;
	rdfs:label "Aggregation Method"@en ;
	rdfs:comment "Method used to aggregate data in presentation of variable"@en .


:CKANIdentifier rdf:type owl:Class ;
	rdfs:label "CKAN Identifier"@en ;
	rdfs:comment "An identifier for this dataset in the CKAN system"@en .


:DataOffset rdf:type owl:Class ;
	rdfs:label "Data Offset"@en ;
	rdfs:comment "An offset specifying the location of a variable in a dataset, such as a column number or byte offset"@en .


:Dataset rdf:type owl:Class ;
	rdfs:subClassOf dcat:Dataset ;
	rdfs:label "Dataset"@en ;
	rdfs:comment "Extension of the W3C Data Catalog dataset that has additional properties for the MINT data catalog"@en .


:MissingValueIndicator rdf:type owl:Class ;
	rdfs:label "Missing Value Indicator"@en ;
	rdfs:comment "The indicator used to denote missing values"@en .

:Presentation rdf:type owl:Class ;
	rdfs:label "Presentation"@en ;
	rdfs:comment "The presentation of a variable in a dataset."@en .

:StandardName rdf:type owl:Class ;
	owl:unionOf (
					geo-upper:Variable
					skos:Concept
				) ;
	rdfs:label "Standard Name"@en ;
	rdfs:comment "A standard name in a domain ontology"@en .

:StoragePath rdf:type owl:Class ;
	rdfs:label "Storage Path"@en ;
	rdfs:comment "The physical or network location of a dataset."@en .

:TimeConvention rdf:type owl:Class ;
	rdfs:label "Time Convention"@en ;
	rdfs:comment "The convention used for modeling time values."@en .

:Variable rdf:type owl:Class ;
	rdfs:label "Variable"@en ;
	rdfs:comment "A Variable with associated datasets stored in the Data Catalog"@en .


